add example of extraction using memory

compiler/examples/extraction-unit-tests/proofs.ec
@@ -1,9 +1,10 @@
-require import AllCore IntDiv.
-from Jasmin require import JUtils JWord.
+require import AllCore IntDiv List.
+from Jasmin require import JUtils JWord JMemory.
 
 require Gcd.
 require Loops.
 require Sdiv.
+require Add_in_mem.
 
 lemma loops_forty_correct : hoare [ Loops.M.forty: true ==> res = W32.of_int 40 ].
 proof. by proc; unroll for ^while; auto. qed.
@@ -39,4 +40,54 @@ proof.
     by rewrite gcd_modl gcdC.
   skip => &m [] /= <- <- _ g' ->.
   by rewrite gcd0z.
+qed.
+
+(* ------------------------------------------------ *)
+
+op to_list (m:global_mem_t) (p len : int) =
+  map (fun i => loadW64 m (p + 8*i)) (iota_ 0 len).
+
+lemma size_to_list m p len : 0 <= len => size (to_list m p len) = len.
+proof. rewrite /to_list size_map size_iota /#. qed.
+
+lemma to_list0 m p : to_list m p 0 = [].
+proof. by rewrite /to_list iota0. qed.
+
+lemma to_listS m p len : 0 <= len => to_list m p (len + 1) = rcons (to_list m p len) (loadW64 m (p + 8*len)).
+proof. by move=> ?; rewrite /to_list iotaSr // map_rcons. qed.
+
+op addl (l1 l2 : W64.t list) = map (fun (p:W64.t * W64.t) => p.`1 + p.`2) (zip l1 l2).
+
+lemma addl_rcons l1 l2 w1 w2 :
+  size l1 = size l2 => addl (rcons l1 w1) (rcons l2 w2) = rcons (addl l1 l2) (w1 + w2).
+proof. by move=> heq; rewrite /addl zip_rcons // map_rcons. qed.
+
+op disjoint_ptr (out inp len : int) = out <= inp || inp + len <= out .
+
+hoare add_mem_correct (m_ : global_mem_t) (out_ in1_ in2_ len_ : int) :
+  Add_in_mem.M.add_mem :
+    Glob.mem = m_ /\ out = out_ /\ in1 = in1_ /\ in2 = in2_ /\ len = len_ /\
+    disjoint_ptr out in1 (8*len) /\ disjoint_ptr out in2 (8*len)
+    ==>
+    to_list Glob.mem out_ len_ = addl (to_list m_ in1_ len_) (to_list m_ in2_ len_).
+proof.
+  proc.
+  case: (len <= 0).
+  + rcondf ^while; auto => />; 1: by smt().
+    by move=> _ _ hlen; rewrite /to_list iota0.
+  while (0 <= i <= len /\
+         out = out_ /\ in1 = in1_ /\ in2 = in2_ /\ len = len_ /\
+         disjoint_ptr out in1 (8*len) /\ disjoint_ptr out in2 (8*len) /\
+         (forall j, i <= j < len => loadW64 Glob.mem (in1 + 8*j) = loadW64 m_ (in1 + 8*j) /\
+                                    loadW64 Glob.mem (in2 + 8*j) = loadW64 m_ (in2 + 8*j)) /\
+         to_list Glob.mem out_ i = addl (to_list m_ in1_ i) (to_list m_ in2_ i)).
+  + auto => /> &hr h0i _ hdisj1 hdisj2 heqm_ hrec hilen.
+    rewrite !to_listS // addl_rcons 1:!size_to_list // -hrec; split; 1: smt().
+    split.
+    + move=> j hij hj; rewrite !store_load64_neq 1, 2:/#.
+      apply: heqm_; smt().
+    congr.
+    + apply List.eq_in_map => j /mem_iota hj /=; rewrite store_load64_neq; smt().
+    by rewrite store_load64_eq; have [-> ->]:= heqm_ i{hr} _.
+  auto => />; smt (to_list0).
 qed.
