eclib/JMemory.ec
@@ -54,7 +54,7 @@ proof. by rewrite storesE. qed.
 
 lemma stores_cons m a w ws : stores m a (w::ws) = stores (m.[a <- w]) (a + 1) ws.
 proof.
-  rewrite !storesE iotaredE /= addrC iotaS 1:List.size_ge0. 
+  rewrite !storesE iotaredE /= addrC iotaS 1:List.size_ge0.
   rewrite (addzC 0 1) iota_addl /=.
   rewrite -(revK (iota_ 0 (size ws))) map_rev !foldl_rev foldr_map /=.
   rewrite -!foldl_rev !revK; apply foldl_in_eq => m0 i /mem_iota /= h.
@@ -95,6 +95,10 @@ op loadW256 (m : global_mem_t) (a : address) =
 lemma loadW32_bits8 m p i : 0 <= i < 4 =>
   loadW32 m p \bits8 i = loadW8 m (p + i).
 proof. by move=> hi;rewrite /loadW32 pack4bE // initiE. qed.
+
+lemma loadW64_bits8 m p i : 0 <= i < 8 =>
+  loadW64 m p \bits8 i = loadW8 m (p + i).
+proof. by move=> hi;rewrite /loadW64 pack8bE // initiE. qed.
 
 lemma loadW128_bits8 m p i : 0 <= i < 16 =>
   loadW128 m p \bits8 i = loadW8 m (p + i).
@@ -138,7 +142,7 @@ proof.
          W4u8.Pack.init (fun i => loadW8 mem (p + i)).
   + by apply W4u8.Pack.all_eqP; rewrite /all_eq.
   apply (can_inj _ _ W4u8.unpack8K); apply W4u8.Pack.packP => i hi.
-  rewrite /loadW32 pack4K //=. 
+  rewrite /loadW32 pack4K //=.
 qed.
 
 lemma load4u32 mem p :
@@ -249,6 +253,20 @@ proof. by rewrite storeW32E !storeW8E storesE /=. qed.
 lemma get_storeW32E m p (w:W32.t) j :
   (storeW32 m p w).[j] = if p <= j < p + 4 then w \bits8 (j - p) else m.[j].
 proof. rewrite storeW32E /= get_storesE /= /#. qed.
+
+lemma store_load64_eq m p w : loadW64 (storeW64 m p w) p = w.
+proof.
+  apply W8u8.wordP => i hi.
+  rewrite loadW64_bits8 // /loadW8 /storeW64 get_storesE size_map /= /#.
+qed.
+
+lemma store_load64_neq m p p' w :
+  p + 8 <= p' || p' + 8 <= p =>
+  loadW64 (storeW64 m p w) p' = loadW64 m p'.
+proof.
+  move=> h; apply W8u8.wordP => i hi.
+  rewrite !loadW64_bits8 // /loadW8 /storeW64 get_storesE size_map /= /#.
+qed.
 
 (* ------------------------------------------------------------------- *)
 (* Global Memory                                                       *)
